% !TEX root=../../main.tex

\onecolumn



\begin{proof}[Proof of Theorem~\ref{thm:notSat}]
  By Definition~\ref{def:Sat}, the premise of Theorem~\ref{thm:notSat}, $\neg\text{SAT }(\phi\land\phi')$,
  means that there does not exist a mapping $M=[s_0\mapsto c_0,\cdots,s_n\mapsto c_n]$ such that $M(\phi\land\phi')\equiv\True$.
  This can be rewritten to for all mappings $M$, $\neg M\phi \lor \neg M\phi'$.

  We now need to show that this implies that there exists no mapping $M$,
  such that $t,M\sigma\xrightarrow[]{Mi}\bar{t'},\bar{\sigma'}\xrightarrow[]{Mi'}\bar{t''},\bar{\sigma''}$.

  By Lemma~\ref{lem:notSatDrive}, etc etc etc \fixme{complete this}
\end{proof}

\begin{lemma}[Unsatisfiable symbolic evaluation]
  \label{lem:notSatEval}
  For all expressions $e$ and states $\sigma$ such that $e,\sigma\eval\overline{v,\sigma',\phi}$, and mappings $M=[s_0\mapsto c_0,\cdots,s_n\mapsto c_n]$ we have $M\phi \iff e,M\sigma\bar{\eval}\bar{v},\bar{\sigma'}$.

\end{lemma}

\begin{proof}[Proof of Lemma~\ref{lem:notSatEval}]
  From Lemma~\ref{lem:soundeval}, we can directly conclude that $\forall M . M\phi \implies e,M\sigma\bar{\eval}\bar{v},\bar{\sigma'}$.\\
  What remains to be proven is $\forall M . e,M\sigma\bar{\eval}\bar{v},\bar{\sigma'}\implies M\phi$.

  We prove this by induction over $e$.\\

  \case{$e=\tuple{e_1,e_2}$}
    {
      One rule applies, namely \userule{Sym-E-Pair}\\
      Provided that \userule{E-Pair} with $\bar{\sigma}=M\sigma$, then from the induction hypothesis, we obtain the following.\\

      $\forall M_1 . e_1,M_1\sigma\bar{\eval}\bar{v_1},\bar{\sigma'}\implies M_1\phi_1$ and\\
      $\forall M_2 . e_2,M_2\sigma'\bar{\eval}\bar{v_2},\bar{\sigma''}\implies M_2\phi_2$\\

      \fixme{how does the proof proceed? We do not know that there exists an $M$ that satsifies both, just that they can be individually satisfied, no?}
    }

\end{proof}

\begin{lemma}[Unsatisfiable symbolic striding]
  \label{lem:notSatStride}
  For all tasks $t$ and states $\sigma$ such that $t,\sigma\stride\overline{t',\sigma',\phi}$, if we have $\neg\text{SAT }(\phi)$ then $\neg\exists M$ such that $t,M\sigma\bar{\stride}\bar{t'},\bar{\sigma'}$

\end{lemma}



\begin{proof}[Proof of Lemma~\ref{lem:notSatStride}]

\end{proof}

\begin{lemma}[Unsatisfiable symbolic normalisation]
  \label{lem:notSatNorm}
  For all expressions $e$ and states $\sigma$ such that $e,\sigma\normalise\overline{t,\sigma',\phi}$, if we have $\neg\text{SAT }(\phi)$ then $\neg\exists M$ such that $e,M\sigma\bar{\normalise}\bar{t},\bar{\sigma'}$

\end{lemma}



\begin{proof}[Proof of Lemma~\ref{lem:notSatNorm}]

\end{proof}

\begin{lemma}[Unsatisfiable symbolic handling]
  \label{lem:notSatHandle}
  For all tasks $t$ and states $\sigma$ such that $t,\sigma\handle{}\overline{t',\sigma',i,\phi}$, if we have $\neg\text{SAT }(\phi)$ then $\neg\exists M$ such that $t,M\sigma\xrightarrow[]{Mi}\bar{t'},\bar{\sigma'}$

\end{lemma}



\begin{proof}[Proof of Lemma~\ref{lem:notSatHandle}]

\end{proof}

\begin{lemma}[Unsatisfiable symbolic driving]
  \label{lem:notSatDrive}
  For all tasks $t$ and states $\sigma$ such that $t,\sigma\drive{}\overline{t',\sigma',i,\phi}$, if we have $\neg\text{SAT }(\phi)$ then $\neg\exists M$ such that $t,M\sigma\xRightarrow[]{Mi}\bar{t'},\bar{\sigma'}$

\end{lemma}

\begin{proof}[Proof of Lemma~\ref{lem:notSatDrive}]

\end{proof}
